

# MATH 238 Homework 6

Brendan Tea

February 23, 2026

## Contents

<b>Homework for Section 4.2: 50 points</b>	<b>1</b>
Problem 4.4.30 . . . . .	1
Problem 4.4.34 . . . . .	3
Problem 4.4.42 . . . . .	4
<b>Homework for Section 4.3: 50 points</b>	<b>7</b>
Problem 4.6.4 . . . . .	7
Problem 4.6.10 . . . . .	8

## Homework for Section 4.4: 50 points

In Problems 27 - 36 solve the given initial-value problem.

### Problem 4.4.30

Given:  $y'' + 4y' + 4y = (3 + x)e^{-2x}$ ;  $y(0) = 2$ ,  $y'(0) = 5$

Find:  $y(x)$

**SOLUTION:** When we are solving for our general solution, we must first solve for our complementary solution, using auxiliary equations, and solve for our particular solution, using the method of undetermined coefficients. Then we can use our IVP to solve for our constants.

Solving auxiliary equation for  $y_c(x)$ .

$$\begin{aligned}y'' + 4y' + 4y &= 0 \\m^2 + 4m + 4 &= 0 \\m &= (m + 2)^2, \quad m = -2, -2 \\ \implies y_c(x) &= C_1 e^{-2x} + C_2 x e^{-2x}\end{aligned}$$

Method of undetermined coefficients for  $y_p(x)$ . Notice how there are multiple repeated roots for  $e^{-2x}$ .

$$\text{Assume: } y_p(x) = x^2(Ax + B)e^{-2x}$$

$$y_p(x) = (Ax^3 + Bx^2)e^{-2x}$$

$$y'_p(x) = (3Ax^2 + 2Bx - 2Ax^3 - 2Bx^2)e^{-2x}$$

$$y'_p(x) = (-2Ax^3 + 3Ax^2 - 2Bx^2 + 2Bx)e^{-2x}$$

$$y''_p(x) = (-6Ax^2 + 6Ax - 4Bx + 2B + 4Ax^3 - 6Ax^2 + 4Bx^2 - 4Bx)e^{-2x}$$

$$y''_p(x) = (4Ax^3 - 12Ax^2 + 4Bx^2 + 6Ax - 8Bx + 2B)e^{-2x}$$

Substitute  $y_p(x)$  and solve for constants.

$$y_p(x)'' + 4y_p(x)' + 4y_p(x) = (3 + x)e^{-2x}$$

$$(4Ax^3 - 12Ax^2 + 4Bx^2 + 6Ax - 8Bx + 2B)e^{-2x} + 4(-2Ax^3 + 3Ax^2 - 2Bx^2 + 2Bx)e^{-2x} + 4(Ax^3 + Bx^2)e^{-2x} = (3 + x)e^{-2x}$$

$$(4Ax^3 - 12Ax^2 + 4Bx^2 + 6Ax - 8Bx + 2B) + (-8Ax^3 + 12Ax^2 - 8Bx^2 + 8Bx) + (4Ax^3 + 4Bx^2) = 3 + x$$

$$6Ax + 2B = 3 + x$$

$$\Rightarrow \begin{cases} 6Ax = x \\ 2B = 3 \end{cases}$$

$$A = \frac{1}{6}, B = \frac{3}{2}$$

$$\Rightarrow \boxed{y_p(x) = \left(\frac{1}{6}x^3 + \frac{3}{2}x^2\right)e^{-2x}}$$

Combine to create  $y_g(x)$ .

$$y_g(x) = y_c(x) + y_p(x)$$

$$\Rightarrow \boxed{y_g(x) = C_1e^{-2x} + C_2xe^{-2x} + \left(\frac{1}{6}x^3 + \frac{3}{2}x^2\right)e^{-2x}}$$

Now we have to solve the IVP and obtain our constants.

$$y(0) = 2, y'(0) = 5$$

$$y_g(x) = C_1e^{-2x} + C_2xe^{-2x} + \left(\frac{1}{6}x^3 + \frac{3}{2}x^2\right)e^{-2x}$$

$$y'_g(x) = -2C_1e^{-2x} + C_2e^{-2x} - 2C_2xe^{-2x} + \left(\frac{1}{2}x^2 + 3x\right)e^{-2x} - 2\left(\frac{1}{6}x^3 + \frac{3}{2}x^2\right)e^{-2x}$$

$$y'_g(x) = -2C_1e^{-2x} + C_2e^{-2x} - 2C_2xe^{-2x} + \left(\frac{1}{2}x^2 + 3x\right)e^{-2x} + \left(-\frac{1}{3}x^3 - 3x^2\right)e^{-2x}$$

Plugging in.

$$y(0) = 2$$

$$y_g(0) = C_1e^{-2(0)} + C_2(0)e^{-2(0)} + \left(\frac{1}{6}(0)^3 + 3(0)^2\right)e^{-2(0)} = 2$$

$$y_g(0) = C_1 = 2$$

$$y'(0) = 5$$

$$y'_g(0) = -2C_1e^{-2(0)} + C_2e^{-2(0)} - 2C_2(0)e^{-2(0)} + \left(\frac{1}{2}(0)^2 + 3(0)\right)e^{-2(0)} + \left(-\frac{1}{3}(0)^3 - 3(0)^2\right)e^{-2(0)} = 5$$

$$y'_g(0) = -2C_1 + C_2 = 5$$

$$y'_g(0) = -2(2) + C_2 = 5$$

$$y'_g(0) = C_2 = 9$$

Combine to create  $y(x)$ .

$$\begin{aligned}
 C_1 &= 2, \quad C_2 = 9 \\
 y_g(x) &= C_1 e^{-2x} + C_2 x e^{-2x} + \left( \frac{1}{6} x^3 + \frac{3}{2} x^2 \right) e^{-2x} \\
 \Rightarrow y_g(x) &= 2e^{-2x} + 9xe^{-2x} + \left( \frac{1}{6} x^3 + \frac{3}{2} x^2 \right) e^{-2x}
 \end{aligned}$$

### Problem 4.4.34

Given:  $\frac{d^2 x}{dt^2} + \omega^2 x = F_0 \cos(\gamma t); \quad x(0) = 0, \quad x'(0) = 0$

Find:  $x(t)$

**SOLUTION:** When we are solving for our general solution, we must first solve for our complementary solution, using auxiliary equations, and solve for our particular solution, using the method of undetermined coefficients. Then we can use our IVP to solve for our constants.

Solving auxiliary equation for  $x_c(t)$ .

$$\begin{aligned}
 \frac{d^2 x}{dt^2} + \omega^2 x &= F_0 \cos \gamma t \\
 m^2 + \omega^2 &= 0 \\
 m &= \pm i\omega \\
 \Rightarrow x_c(t) &= C_1 \cos(\omega t) + C_2 \sin(\omega t)
 \end{aligned}$$

Method of undetermined coefficients for  $x_p(t)$ .

$$\begin{aligned}
 \text{Assume: } x_p(t) &= A \cos(\gamma t) + B \sin(\gamma t) \\
 x_p'(t) &= -\gamma A \sin(\gamma t) + \gamma B \cos(\gamma t) \\
 x_p''(t) &= -\gamma^2 A \cos(\gamma t) - \gamma^2 B \sin(\gamma t)
 \end{aligned}$$

Substitute  $x_p(t)$  and solve for constants.

$$\begin{aligned}
 \frac{d^2 x_p(t)}{dt^2} + \omega^2 x_p(t) &= F_0 \cos(\gamma t) \\
 (-\gamma^2 A \cos(\gamma t) - \gamma^2 B \sin(\gamma t)) + \omega^2 (A \cos(\gamma t) + B \sin(\gamma t)) &= F_0 \cos(\gamma t) \\
 (-\gamma^2 A \cos(\gamma t) - \gamma^2 B \sin(\gamma t)) + (\omega^2 A \cos(\gamma t) + \omega^2 B \sin(\gamma t)) &= F_0 \cos(\gamma t) \\
 A(\omega^2 - \gamma^2) \cos(\gamma t) + B(\omega^2 - \gamma^2) \sin(\gamma t) &= F_0 \cos(\gamma t) \\
 \Rightarrow \begin{cases} A(\omega^2 - \gamma^2) \cos(\gamma t) = F_0 \cos(\gamma t) \\ B(\omega^2 - \gamma^2) \sin(\gamma t) = 0 \end{cases} \\
 A = \frac{F_0}{\omega^2 - \gamma^2}, \quad B = 0 \\
 \Rightarrow x_p(t) = \frac{F_0}{\omega^2 - \gamma^2} \cos(\gamma t)
 \end{aligned}$$

Combine to create  $x_g(t)$ .

$$x_g(t) = x_c(t) + x_p(t)$$

$$\Rightarrow x_g(t) = C_1 \cos(\omega t) + C_2 \sin(\omega t) + \frac{F_0}{\omega^2 - \gamma^2} \cos(\gamma t)$$

Now we have to solve the IVP and obtain our constants.

$$x(0) = 0, \quad x'(0) = 0$$

$$x_g(t) = C_1 \cos(\omega t) + C_2 \sin(\omega t) + \frac{F_0}{\omega^2 - \gamma^2} \cos(\gamma t)$$

$$x'_g(t) = -\omega C_1 \sin(\omega t) + \omega C_2 \cos(\omega t) - \frac{F_0 \gamma}{\omega^2 - \gamma^2} \sin(\gamma t)$$

Plugging in.

$$x_g(0) = C_1 + \frac{F_0}{\omega^2 - \gamma^2} = 0$$

$$x_g(0) = C_1 = -\frac{F_0}{\omega^2 - \gamma^2}$$

$$x'_g(0) = -\omega C_1 \sin(\omega(0)) + \omega C_2 \cos(\omega(0)) - \frac{F_0 \gamma}{\omega^2 - \gamma^2} \sin(\gamma(0))$$

$$x'_g(0) = \omega C_2 = 0$$

$$x'_g(0) = C_2 = 0$$

Combine to create  $x(t)$ .

$$C_1 = -\frac{F_0}{\omega^2 - \gamma^2}, \quad C_2 = 0$$

$$x_g(t) = C_1 \cos(\omega t) + C_2 \sin(\omega t) + \frac{F_0}{\omega^2 - \gamma^2} \cos(\gamma t)$$

$$x(t) = -\frac{F_0}{\omega^2 - \gamma^2} \cos(\omega t) + \frac{F_0}{\omega^2 - \gamma^2} \cos(\gamma t)$$

$$\Rightarrow x(t) = \frac{F_0}{\omega^2 - \gamma^2} (\cos(\gamma t) - \cos(\omega t))$$

#### Problem 4.4.42

In Problems 41 and 42 solve the given initial-value problem in which the input function  $g(x)$  is discontinuous. [Hint: Solve each problem on two intervals, and then find a solution so that  $y$  and  $y'$  are continuous at  $x = \pi/2$  (Problem 41) and  $x = \pi$  (Problem 42)]

Given:  $y'' - 2y' + 10y = g(x)$ ,  $y(0) = 0$ ,  $y'(0) = 0$ , where

$$g(x) = \begin{cases} 20 & 0 \leq x \leq \pi \\ 0 & x > \pi \end{cases}$$

Find:  $y(x)$

**SOLUTION:** This problem is unique as it is two nonhomogenous problems in one. We will solve both general solutions normally as the past two. We will be able to find our first set of constants for the range of  $0 \leq x \leq \pi$  by just normally

plugging in. For the range of  $x \geq \pi$ , we will have to make it satisfy continuity and smoothness continuity. In other words,  $y_1(\pi) = y_2(\pi)$  for continuity and  $y_1'(\pi) = y_2'(\pi)$  for smoothness.

Solving for  $y_{1c}(x)$  for range of  $0 \leq x \leq \pi$ .

$$\begin{aligned}
y'' - 2y' + 10y &= 20 \\
m^2 - 2m + 10 &= 0 \\
m &= \frac{2 \pm \sqrt{4 - 40}}{2} \\
m &= \frac{2 \pm 6i}{2} \\
m &= 1 + 3i, 1 - 3i \\
\Rightarrow y_{1c}(x) &= e^x (C_1 \cos(3x) + C_2 \sin(3x))
\end{aligned}$$

Solving for  $y_{1p}(x)$  for range of  $0 \leq x \leq \pi$ .

$$\begin{aligned}
\text{Assume: } y_{1p}(x) &= A \\
y_{1p}^{(n)}(x) &= 0, \quad n \in \mathbb{Z}^+, \quad n \geq 1 \\
y_p'' - 2y_p' + 10y_p &= 20 \\
10A &= 20 \\
A &= 2 \\
\Rightarrow y_{1p}(x) &= 2
\end{aligned}$$

Solving for  $y_{1g}(x)$  and  $y_{1g}'(x)$ .

$$\begin{aligned}
y_{1g}(x) &= y_{1c}(x) + y_{1p}(x) \\
y_{1g}(x) &= e^x (C_1 \cos(3x) + C_2 \sin(3x)) + 2 \\
y_{1g}'(x) &= e^x (C_1 \cos(3x) + C_2 \sin(3x)) + e^x (-3C_1 \sin(3x) + 3C_2 \cos(3x)) \\
y_{1g}'(x) &= e^x ((C_1 + 3C_2) \cos(3x) + (C_2 - 3C_1) \sin(3x))
\end{aligned}$$

Plugging in for constants.

$$\begin{aligned}
y(0) &= 0, \quad y'(0) = 0 \\
y_{1g}(0) &= \cancel{e^0} (C_1 \cos(3(0)) + \cancel{C_2 \sin(3(0))}) + 2 = 0 \\
y_{1g}(0) &= C_1 + 2 = 0 \\
y_{1g}(0) &= C_1 = -2 \\
y_{1g}'(0) &= \cancel{e^0} \left( (C_1 + 3C_2) \cos(3(0)) + \cancel{(C_2 - 3C_1) \sin(3(0))} \right) = 0 \\
y_{1g}'(0) &= C_1 + 3C_2 = 0 \\
y_{1g}'(0) &= (-2) + 3C_2 = 0 \\
y_{1g}'(0) &= C_2 = \frac{2}{3}
\end{aligned}$$

Combine for  $y_1(x)$  for range of  $0 \leq x \leq \pi$ .

$$\begin{aligned}
C_1 &= -2, \quad C_2 = \frac{2}{3} \\
y_{1g}(x) &= e^x (C_1 \cos(3x) + C_2 \sin(3x)) + 2 \\
\Rightarrow y_1(x) &= e^x \left( -2 \cos(3x) + \frac{2}{3} \sin(3x) \right) + 2
\end{aligned}$$

Now the same thing for  $y_2(x)$  for the range of  $x > \pi$ . We should recognize this is just the homogenous, complementary part from  $y_1(x)$  so we can skip and state the following. There is no particular solution as it is homogenous.

$$\begin{aligned}
 y'' - 2y' + 10y &= 0 \\
 \implies y_{2g}(x) &= y_{1c}(x) \\
 \boxed{y_{2g}(x) &= e^x (C_3 \cos(3x) + C_4 \sin(3x))}
 \end{aligned}$$

Now have to have to satisfy continuity and smoothness continuity for our constants.

$$\begin{aligned}
 y_1(\pi) &= y_2(\pi) \\
 y_1(x) &= e^x \left( -2 \cos(3x) + \frac{2}{3} \sin(3x) \right) + 2 \\
 y_1(x) &= e^{(\pi)} \left( -2 \cos(3(\pi)) + \frac{2}{3} \sin(3(\pi)) \right) + 2 \\
 y_1(\pi) &= 2e^\pi + 2 \\
 y_2(x) &= e^x (C_3 \cos(3x) + C_4 \sin(3x)) \\
 y_2(\pi) &= e^{(\pi)} (C_3 \cos(3(\pi)) + \cancel{C_4 \sin(3(\pi))}) \\
 y_2(\pi) &= -C_3 e^\pi \\
 y_1(\pi) &= y_2(\pi) \\
 2e^\pi + 2 &= -C_3 e^\pi \\
 C_3 &= -2 - 2e^{-\pi} \\
 \\ 
 y'_1(\pi) &= y'_2(\pi) \\
 y'_1(x) &= e^x ((C_1 + 3C_2) \cos(3x) + (C_2 - 3C_1) \sin(3x)) \\
 y'_1(x) &= e^{(\pi)} ((C_1 + 3C_2) \cos(3(\pi)) + \cancel{(C_2 - 3C_1) \sin(3(\pi))}) \\
 y'_1(\pi) &= -e^\pi (C_1 + 3C_2) \\
 y'_1(\pi) &= -e^\pi \left( -2 + 3\frac{2}{3} \right) \\
 y'_1(\pi) &= 0 \\
 y'_2(x) &= e^x ((C_3 + 3C_4) \cos(3x) + (C_3 - 3C_4) \sin(3x)) \\
 y'_2(\pi) &= -e^\pi (C_3 + 3C_4) \\
 y'_1(\pi) &= y'_2(\pi) \\
 0 &= \cancel{e^\pi} (C_3 + 3C_4) \\
 0 &= -2 - 2e^{-\pi} + 3C_4 \\
 C_4 &= \frac{2 + 2e^{-\pi}}{3}
 \end{aligned}$$

$$\begin{aligned}
 y_{2g}(x) &= e^x (C_3 \cos(3x) + C_4 \sin(3x)) \\
 y_2(x) &= e^x \left( (-2 - 2e^{-\pi}) \cos(3x) + \left( \frac{2 + 2e^{-\pi}}{3} \right) \sin(3x) \right) \\
 \implies \boxed{y_2(x) &= e^x (1 + e^{-\pi}) \left( -2 \cos(3x) + \frac{2}{3} \sin(3x) \right)}
 \end{aligned}$$

Combining everything.

$$\Rightarrow y(x) = \begin{cases} e^x (-2 \cos(3x) + \frac{2}{3} \sin(3x)) + 2 & 0 \leq x \leq \pi \\ e^x (1 + e^{-\pi}) (-2 \cos(3x) + \frac{2}{3} \sin(3x)) & x > \pi \end{cases}$$

## Homework for Section 4.6: 50 points

In Problems 1 - 20 solve each differential equation by variation of parameters.

For second order, we will assume our particular solution comes in this form.

$$y_p(x) = u_1 y_1 + u_2 y_2 \quad (1)$$

After a process, we will arrive with these pairs of equations.

$$\begin{aligned} \text{Assume: } u_1'(x) y_1(x) + u_2'(x) y_2(x) &= 0 \\ \Rightarrow u_1'(x) y_1'(x) + u_2'(x) y_2'(x) &= f(x) \end{aligned}$$

By Cramer's Rule.

$$u_1'(x) = \frac{W_1}{W} \quad (2)$$

$$u_2'(x) = \frac{W_2}{W} \quad (3)$$

### Problem 4.6.4

Given:  $y'' + y = \sec \theta \tan \theta$

Find:  $y_g(\theta)$

**SOLUTION:** We simply use auxiliary equations for our complimentary equation and Cramer's rule to find our  $u_1'$  and  $u_2'$  to find our particular solution  $y_p(\theta)$ .

Solving for  $y_c(x)$ .

$$\begin{aligned} y'' + y &= \sec \theta \tan \theta \\ m^2 + 1 &= 0 \\ m &= \pm i \\ \Rightarrow y_c(\theta) &= C_1 \cos(\theta) + C_2 \sin(\theta) \end{aligned}$$

Solving for determinants  $W$ ,  $W_1$ ,  $W_2$ .

$$\begin{aligned} y_p(\theta) &= u_1 y_1 + u_2 y_2 \\ y_1(\theta) &= \cos(\theta), \quad y_2(\theta) = \sin(\theta), \quad f(\theta) = \sec \theta \tan \theta \\ W &= \begin{vmatrix} \cos(\theta) & \sin(\theta) \\ -\sin(\theta) & \cos(\theta) \end{vmatrix} = 1 \\ W_1 &= \begin{vmatrix} 0 & \sin(\theta) \\ \sec \theta \tan \theta & \cos(\theta) \end{vmatrix} = -\tan^2(\theta) \\ W_2 &= \begin{vmatrix} \cos(\theta) & 0 \\ -\sin(\theta) & \sec \theta \tan \theta \end{vmatrix} = \tan(\theta) \end{aligned}$$

Solving for  $u_1(\theta)$  and  $u_2(\theta)$ .

$$u_1(\theta) = \int \frac{W_1}{W} d\theta$$

$$u_1(\theta) = \int -\tan^2(\theta) d\theta$$

$$u_1(\theta) = \int (1 - \sec^2(\theta)) d\theta$$

$$u_1(\theta) = \theta - \tan(\theta)$$

$$u_2(\theta) = \int \frac{W_2}{W} d\theta$$

$$u_2(\theta) = \int \tan(\theta) d\theta$$

$$u_2(\theta) = \ln |\sec(\theta)|$$

Solving for  $y_p(\theta)$ .

$$y_p(x) = u_1 y_1 + u_2 y_2$$

$$y_p(x) = (\theta - \tan(\theta)) (\cos(\theta)) + (\ln |\sec(\theta)|) (\sin(\theta))$$

$$y_p(x) = \theta \cos(\theta) - \sin(\theta) + \sin(\theta) \ln |\sec(\theta)|$$

Now combine and sum  $y_c$  and  $y_p$ . Additionally, see how there is a repeated solution  $\sin(\theta)$  that will get swallowed up by constant in  $y_c$ .

$$y_g(\theta) = y_c(\theta) + y_p(\theta)$$

$$y_g(\theta) = C_1 \cos(\theta) + C_2 \sin(\theta) + \theta \cos(\theta) - \sin(\theta) + \sin(\theta) \ln |\sec(\theta)|$$

$$\Rightarrow \boxed{y_g(\theta) = C_1 \cos(\theta) + C_2 \sin(\theta) + \theta \cos(\theta) + \sin(\theta) \ln |\sec(\theta)|}$$

### Problem 4.6.10

Given:  $4y'' - y = e^{\frac{x}{2}} + 3$

Find:  $y_g(x)$

**SOLUTION:** We simply use auxiliary equations for our complimentary equation and Cramer's rule to find our  $u'_1$  and  $u'_2$  to find our particular solution  $y_p(x)$ .

Solving for  $y_c(x)$ .

$$4y'' - y = e^{\frac{x}{2}} + 3$$

$$4m^2 - 1 = 0$$

$$m = \pm \frac{1}{2}$$

$$\Rightarrow \boxed{y_c(x) = C_1 e^{\frac{x}{2}} + C_2 e^{-\frac{x}{2}}}$$



Solving for determinants  $W$ ,  $W_1$ ,  $W_2$ .

$$\begin{aligned}
y_p(x) &= u_1 y_1 + u_2 y_2 \\
y_1(x) &= e^{\frac{x}{2}}, \quad y_2(x) = e^{-\frac{x}{2}}, \quad f(x) = \frac{e^{\frac{x}{2}} + 3}{4} \\
W &= \begin{vmatrix} e^{\frac{x}{2}} & e^{-\frac{x}{2}} \\ \frac{1}{2}e^{\frac{x}{2}} & -\frac{1}{2}e^{-\frac{x}{2}} \end{vmatrix} \\
W &= e^{\frac{x}{2}} e^{-\frac{x}{2}} \begin{vmatrix} 1 & 1 \\ \frac{1}{2} & -\frac{1}{2} \end{vmatrix} = -1 \\
W_1 &= \begin{vmatrix} 0 & e^{-\frac{x}{2}} \\ \frac{e^{\frac{x}{2}} + 3}{4} & -\frac{1}{2}e^{-\frac{x}{2}} \end{vmatrix} \\
W_1 &= e^{-\frac{x}{2}} \begin{vmatrix} 0 & 1 \\ \frac{e^{\frac{x}{2}} + 3}{4} & -\frac{1}{2} \end{vmatrix} = -\frac{1 + 3e^{-\frac{x}{2}}}{4} \\
W_2 &= \begin{vmatrix} e^{\frac{x}{2}} & 0 \\ \frac{1}{2}e^{\frac{x}{2}} & \frac{e^{\frac{x}{2}} + 3}{4} \end{vmatrix} \\
W_2 &= e^{\frac{x}{2}} \begin{vmatrix} 1 & 0 \\ \frac{1}{2} & \frac{e^{\frac{x}{2}} + 3}{4} \end{vmatrix} \\
W_2 &= e^{\frac{1}{2}x} \left( \frac{1 + 3e^{\frac{x}{2}}}{4} \right) \\
W_2 &= \frac{e^x + 3e^{\frac{x}{2}}}{4}
\end{aligned}$$

Solving for  $u_1(x)$  and  $u_2(x)$ .

$$\begin{aligned}
u_1(x) &= \int \frac{W_1}{W} dx \\
u_1(x) &= \int \frac{3e^{-\frac{x}{2}} + 1}{4} dx \\
u_1(x) &= \frac{x - 6e^{-\frac{x}{2}}}{4} \\
u_2(x) &= \int \frac{W_2}{W} dx \\
u_2(x) &= \int \frac{-e^x - 3e^{\frac{x}{2}}}{4} dx \\
u_2(x) &= \frac{-e^x - 6e^{\frac{x}{2}}}{4}
\end{aligned}$$

Solving for  $y_p(x)$ .

$$\begin{aligned}
y_p(x) &= u_1 y_1 + u_2 y_2 \\
y_p(x) &= \left( \frac{x - 6e^{-\frac{x}{2}}}{4} \right) (e^{\frac{x}{2}}) + \left( \frac{-e^x - 6e^{\frac{x}{2}}}{4} \right) (e^{-\frac{x}{2}}) \\
y_p(x) &= \frac{x e^{\frac{x}{2}}}{4} - \frac{6}{4} - \frac{e^{\frac{x}{2}}}{4} - \frac{6}{4} \\
y_p(x) &= \frac{x e^{\frac{x}{2}}}{4} - \frac{e^{\frac{x}{2}}}{4} - 3
\end{aligned}$$

Now combine and sum  $y_c$  and  $y_p$ . Additionally, see how there is a repeated solution  $-e^{\frac{x}{2}}/4$  that will get swallowed up by

constant in  $y_c$ .

$$\begin{aligned}
 y_g(x) &= y_c(x) + y_p(x) \\
 y_g(x) &= C_1 e^{\frac{x}{2}} + C_2 e^{-\frac{x}{2}} + \frac{x e^{\frac{x}{2}}}{4} - \cancel{\frac{e^{\frac{x}{2}}}{4}} - 3 \\
 \implies \boxed{y_g(x) &= C_1 e^{\frac{x}{2}} + C_2 e^{-\frac{x}{2}} + \frac{x e^{\frac{x}{2}}}{4} - 3}
 \end{aligned}$$